James C - add, sub, and, or, not also done

StackToAssembly.thy
@@ -11,7 +11,7 @@ primrec instruction_conv :: "stack_instruction \<Rightarrow> assembly list" wher
 | "instruction_conv Lt = undefined"
 | "instruction_conv And = [CAssm {A} (Reg M), CAssm {D} (Reg M), AAssm 0, CAssm {A, M} (Decr M), CAssm {M} DAndM, AAssm 0]"
 | "instruction_conv Or = [CAssm {A} (Reg M), CAssm {D} (Reg M), AAssm 0, CAssm {A, M} (Decr M), CAssm {M} DOrM, AAssm 0]"
-| "instruction_conv Not = [CAssm {A} (Reg M), CAssm {D} (NotR M), AAssm 0]"
+| "instruction_conv Not = [CAssm {A} (Reg M), CAssm {M} (NotR M), AAssm 0]"
 
 definition program_convert :: "stack_program \<Rightarrow> assembly_program" where
   "program_convert \<Pi> = map_option concat o map_option (map instruction_conv) o \<Pi>"
@@ -19,9 +19,9 @@ definition program_convert :: "stack_program \<Rightarrow> assembly_program" whe
 primrec stack_to_mem :: "int list \<Rightarrow> (int \<Rightarrow> int) \<Rightarrow> int \<Rightarrow> int" where
   "stack_to_mem [] \<mu> k = (if k = 0 then 0 else \<mu> k)"
 | "stack_to_mem (i # is) \<mu> k = (
-    if k = 0 then 1 + int (length is) 
-    else if k > 0 \<and> k = 1 + int (length is) then i 
-    else stack_to_mem is \<mu> k)" 
+    if k = 0 then 1 + int (length is)
+    else if k = 1 + int (length is) then i
+    else stack_to_mem is \<mu> k)"
 
 primrec state_convert :: "stack_state \<Rightarrow> assembly_state set" where
   "state_convert (\<sigma>, \<pi>) = {(stack_to_mem \<sigma> \<mu>, Some 0, d, concat (map instruction_conv \<pi>)) | d \<mu>. True }"
@@ -31,21 +31,95 @@ primrec state_convert :: "stack_state \<Rightarrow> assembly_state set" where
 lemma [simp]: "dom (program_convert \<Pi>) = dom \<Pi>"
   by (auto simp add: program_convert_def)
 
-lemma [simp]: "(stack_to_mem (i1 # \<sigma>) \<mu>)(1 + int (length \<sigma>) := i2) = stack_to_mem (i2 # \<sigma>) \<mu>"
-  by auto
+lemma [simp]: "k < 0 \<Longrightarrow> stack_to_mem \<sigma> \<mu> k = \<mu> k"
+  by (induction \<sigma>) simp_all
+
+lemma stack_same: "k > 0 \<Longrightarrow> k \<le> int (length \<sigma>) \<Longrightarrow> stack_to_mem \<sigma> \<mu> k = stack_to_mem \<sigma> \<mu>' k"
+  by (induction \<sigma>) simp_all
+
+lemma [simp]: "k > int (length \<sigma>) \<Longrightarrow> stack_to_mem \<sigma> \<mu> k = \<mu> k"
+  by (induction \<sigma>) simp_all
+
+lemma [simp]: "(stack_to_mem (i2 # i3 # \<sigma>) \<mu>)(0 := 1 + int (length \<sigma>), 1 + int (length \<sigma>) := i1) =
+    stack_to_mem (i1 # \<sigma>) (stack_to_mem (i2 # i3 # \<sigma>) \<mu>)"
+  proof
+    fix x
+    show "((stack_to_mem (i2 # i3 # \<sigma>) \<mu>)(0 := 1 + int (length \<sigma>), 1 + int (length \<sigma>) := i1)) x = 
+        stack_to_mem (i1 # \<sigma>) (stack_to_mem (i2 # i3 # \<sigma>) \<mu>) x" 
+      proof (cases "x < 0")
+      case True
+        thus ?thesis by simp
+      next case False
+        with stack_same show ?thesis by (cases "x > int (length \<sigma>)") simp_all
+      qed
+  qed
 
 lemma eval_stack_conv [simp]: "eval_stack \<Pi> \<Sigma>\<^sub>S = Some \<Sigma>\<^sub>S' \<Longrightarrow> \<Sigma>\<^sub>A \<in> state_convert \<Sigma>\<^sub>S \<Longrightarrow> 
     \<exists>\<Sigma>\<^sub>A'. \<Sigma>\<^sub>A' \<in> state_convert \<Sigma>\<^sub>S' \<and> iterate (eval_assembly (program_convert \<Pi>)) \<Sigma>\<^sub>A \<Sigma>\<^sub>A'"
   proof (induction \<Pi> \<Sigma>\<^sub>S rule: eval_stack.induct)
   case (1 \<Pi> i1 i2 \<sigma> \<pi>)
-    thus ?case by simp
-  next case 2
-    thus ?case by simp
+    let ?\<pi>' = "concat (map instruction_conv \<pi>)"
+    from 1 obtain d \<mu> where M: "\<Sigma>\<^sub>A = (stack_to_mem (i1 # i2 # \<sigma>) \<mu>, Some 0, d, 
+      [CAssm {A} (Reg M), CAssm {D} (Reg M), AAssm 0, 
+       CAssm {A, M} (Decr M), CAssm {M} DPlusM, AAssm 0] @ ?\<pi>')" by fastforce
+    from 1 have S: "\<Sigma>\<^sub>S' = ((i1 + i2) # \<sigma>, \<pi>)" by auto
+    let ?\<mu> = "stack_to_mem (i1 # i2 # \<sigma>) \<mu>"
+    let ?\<mu>' = "stack_to_mem ((i1 + i2) # \<sigma>) ?\<mu>"
+    let ?\<Sigma>\<^sub>A\<^sub>1 = "(?\<mu>, Some (?\<mu> 0), d, 
+      [CAssm {D} (Reg M), AAssm 0, CAssm {A, M} (Decr M), CAssm {M} DPlusM, AAssm 0] @ ?\<pi>')"
+    let ?\<Sigma>\<^sub>A\<^sub>2 = "(?\<mu>, Some (?\<mu> 0), ?\<mu> (?\<mu> 0), 
+      [AAssm 0, CAssm {A, M} (Decr M), CAssm {M} DPlusM, AAssm 0] @ ?\<pi>')"
+    let ?\<Sigma>\<^sub>A\<^sub>3 = "(?\<mu>, Some 0, ?\<mu> (?\<mu> 0), [CAssm {A, M} (Decr M), CAssm {M} DPlusM, AAssm 0] @ ?\<pi>')"
+    let ?\<Sigma>\<^sub>A\<^sub>4 = "(?\<mu>(0 := ?\<mu> 0 - 1), Some (?\<mu> 0 - 1), ?\<mu> (?\<mu> 0), [CAssm {M} DPlusM, AAssm 0] @ ?\<pi>')"
+    let ?\<Sigma>\<^sub>A\<^sub>5 = "(?\<mu>', Some (?\<mu> 0 - 1), ?\<mu> (?\<mu> 0), [AAssm 0] @ ?\<pi>')"
+    let ?\<Sigma>\<^sub>A\<^sub>6 = "(?\<mu>', Some 0, ?\<mu> (?\<mu> 0), ?\<pi>')"
+    from M have step1: "eval_assembly (program_convert \<Pi>) \<Sigma>\<^sub>A = Some ?\<Sigma>\<^sub>A\<^sub>1" by simp
+    have step2: "eval_assembly (program_convert \<Pi>) ?\<Sigma>\<^sub>A\<^sub>1 = Some ?\<Sigma>\<^sub>A\<^sub>2" by simp
+    have step3: "eval_assembly (program_convert \<Pi>) ?\<Sigma>\<^sub>A\<^sub>2 = Some ?\<Sigma>\<^sub>A\<^sub>3" by simp
+    have step4: "eval_assembly (program_convert \<Pi>) ?\<Sigma>\<^sub>A\<^sub>3 = Some ?\<Sigma>\<^sub>A\<^sub>4" by (simp add: Let_def)
+    have step5: "eval_assembly (program_convert \<Pi>) ?\<Sigma>\<^sub>A\<^sub>4 = Some ?\<Sigma>\<^sub>A\<^sub>5" by simp
+    have step6: "eval_assembly (program_convert \<Pi>) ?\<Sigma>\<^sub>A\<^sub>5 = Some ?\<Sigma>\<^sub>A\<^sub>6" by simp
+    from iter_two iter_prestep step1 step2 step3 have
+      "iterate (eval_assembly (program_convert \<Pi>)) \<Sigma>\<^sub>A ?\<Sigma>\<^sub>A\<^sub>3" by fast
+    moreover from iter_two iter_prestep step4 step5 step6 have
+      "iterate (eval_assembly (program_convert \<Pi>)) ?\<Sigma>\<^sub>A\<^sub>3 ?\<Sigma>\<^sub>A\<^sub>6" by fast
+    ultimately have X: "iterate (eval_assembly (program_convert \<Pi>)) \<Sigma>\<^sub>A ?\<Sigma>\<^sub>A\<^sub>6" by fast
+    have "?\<Sigma>\<^sub>A\<^sub>6 \<in> state_convert ((i1 + i2) # \<sigma>, \<pi>)" by auto
+    with X S M show ?case by metis
+  next case (2 \<Pi> i1 i2 \<sigma> \<pi>)
+    let ?\<pi>' = "concat (map instruction_conv \<pi>)"
+    from 2 obtain d \<mu> where M: "\<Sigma>\<^sub>A = (stack_to_mem (i1 # i2 # \<sigma>) \<mu>, Some 0, d, 
+      [CAssm {A} (Reg M), CAssm {D} (Reg M), AAssm 0, 
+       CAssm {A, M} (Decr M), CAssm {M} MMinusD, AAssm 0] @ ?\<pi>')" by fastforce
+    from 2 have S: "\<Sigma>\<^sub>S' = ((i2 - i1) # \<sigma>, \<pi>)" by simp
+    let ?\<mu> = "stack_to_mem (i1 # i2 # \<sigma>) \<mu>"
+    let ?\<mu>' = "stack_to_mem ((i2 - i1) # \<sigma>) ?\<mu>"
+    let ?\<Sigma>\<^sub>A\<^sub>1 = "(?\<mu>, Some (?\<mu> 0), d, 
+      [CAssm {D} (Reg M), AAssm 0, CAssm {A, M} (Decr M), CAssm {M} MMinusD, AAssm 0] @ ?\<pi>')"
+    let ?\<Sigma>\<^sub>A\<^sub>2 = "(?\<mu>, Some (?\<mu> 0), ?\<mu> (?\<mu> 0), 
+      [AAssm 0, CAssm {A, M} (Decr M), CAssm {M} MMinusD, AAssm 0] @ ?\<pi>')"
+    let ?\<Sigma>\<^sub>A\<^sub>3 = "(?\<mu>, Some 0, ?\<mu> (?\<mu> 0), [CAssm {A, M} (Decr M), CAssm {M} MMinusD, AAssm 0] @ ?\<pi>')"
+    let ?\<Sigma>\<^sub>A\<^sub>4 = "(?\<mu>(0 := ?\<mu> 0 - 1), Some (?\<mu> 0 - 1), ?\<mu> (?\<mu> 0), [CAssm {M} MMinusD, AAssm 0] @ ?\<pi>')"
+    let ?\<Sigma>\<^sub>A\<^sub>5 = "(?\<mu>', Some (?\<mu> 0 - 1), ?\<mu> (?\<mu> 0), [AAssm 0] @ ?\<pi>')"
+    let ?\<Sigma>\<^sub>A\<^sub>6 = "(?\<mu>', Some 0, ?\<mu> (?\<mu> 0), ?\<pi>')"
+    from M have step1: "eval_assembly (program_convert \<Pi>) \<Sigma>\<^sub>A = Some ?\<Sigma>\<^sub>A\<^sub>1" by simp
+    have step2: "eval_assembly (program_convert \<Pi>) ?\<Sigma>\<^sub>A\<^sub>1 = Some ?\<Sigma>\<^sub>A\<^sub>2" by simp
+    have step3: "eval_assembly (program_convert \<Pi>) ?\<Sigma>\<^sub>A\<^sub>2 = Some ?\<Sigma>\<^sub>A\<^sub>3" by simp
+    have step4: "eval_assembly (program_convert \<Pi>) ?\<Sigma>\<^sub>A\<^sub>3 = Some ?\<Sigma>\<^sub>A\<^sub>4" by (simp add: Let_def)
+    have step5: "eval_assembly (program_convert \<Pi>) ?\<Sigma>\<^sub>A\<^sub>4 = Some ?\<Sigma>\<^sub>A\<^sub>5" by simp
+    have step6: "eval_assembly (program_convert \<Pi>) ?\<Sigma>\<^sub>A\<^sub>5 = Some ?\<Sigma>\<^sub>A\<^sub>6" by simp
+    from iter_two iter_prestep step1 step2 step3 have
+      "iterate (eval_assembly (program_convert \<Pi>)) \<Sigma>\<^sub>A ?\<Sigma>\<^sub>A\<^sub>3" by fast
+    moreover from iter_two iter_prestep step4 step5 step6 have
+      "iterate (eval_assembly (program_convert \<Pi>)) ?\<Sigma>\<^sub>A\<^sub>3 ?\<Sigma>\<^sub>A\<^sub>6" by fast
+    ultimately have X: "iterate (eval_assembly (program_convert \<Pi>)) \<Sigma>\<^sub>A ?\<Sigma>\<^sub>A\<^sub>6" by fast
+    have "?\<Sigma>\<^sub>A\<^sub>6 \<in> state_convert ((i2 - i1) # \<sigma>, \<pi>)" by auto
+    with X S M show ?case by metis
   next case (3 \<Pi> i1 \<sigma> \<pi>)
     let ?\<pi>' = "concat (map instruction_conv \<pi>)"
     from 3 obtain d \<mu> where M: "\<Sigma>\<^sub>A = (stack_to_mem (i1 # \<sigma>) \<mu>, Some 0, d, 
       [CAssm {A} (Reg M), CAssm {M} (NegR M), AAssm 0] @ ?\<pi>')" by fastforce
-    from 3 have S: "\<Sigma>\<^sub>S' = ((-i1) # \<sigma>, \<pi>)" by simp
+    from 3 have S: "\<Sigma>\<^sub>S' = (-i1 # \<sigma>, \<pi>)" by simp
     let ?\<mu> = "stack_to_mem (i1 # \<sigma>) \<mu>"
     let ?\<Sigma>\<^sub>A\<^sub>1 = "(?\<mu>, Some (?\<mu> 0), d, [CAssm {M} (NegR M), AAssm 0] @ ?\<pi>')"
     let ?\<Sigma>\<^sub>A\<^sub>2 = "(?\<mu>(?\<mu> 0 := - ?\<mu> (?\<mu> 0)), Some (?\<mu> 0), d, [AAssm 0] @ ?\<pi>')"
@@ -55,7 +129,8 @@ lemma eval_stack_conv [simp]: "eval_stack \<Pi> \<Sigma>\<^sub>S = Some \<Sigma>
     have "eval_assembly (program_convert \<Pi>) ?\<Sigma>\<^sub>A\<^sub>2 = Some ?\<Sigma>\<^sub>A\<^sub>3" by simp
     with iter_two iter_prestep step1 step2 have X:
       "iterate (eval_assembly (program_convert \<Pi>)) \<Sigma>\<^sub>A ?\<Sigma>\<^sub>A\<^sub>3" by fast
-    have "?\<Sigma>\<^sub>A\<^sub>3 \<in> state_convert ((-i1) # \<sigma>, \<pi>)" by auto
+    have "(stack_to_mem (i1 # \<sigma>) \<mu>)(1 + int (length \<sigma>) := - i1) = stack_to_mem (- i1 # \<sigma>) \<mu>" by auto
+    hence "?\<Sigma>\<^sub>A\<^sub>3 \<in> state_convert ((-i1) # \<sigma>, \<pi>)" by auto
     with X S M show ?case by metis
   next case 4
     thus ?case by simp
@@ -63,15 +138,86 @@ lemma eval_stack_conv [simp]: "eval_stack \<Pi> \<Sigma>\<^sub>S = Some \<Sigma>
     thus ?case by simp
   next case 6
     thus ?case by simp
-  next case 7
-    thus ?case by simp
-  next case 8
-    thus ?case by simp
-  next case 9
-    thus ?case by simp
+  next case (7 \<Pi> i1 i2 \<sigma> \<pi>)
+    let ?\<pi>' = "concat (map instruction_conv \<pi>)"
+    from 7 obtain d \<mu> where M: "\<Sigma>\<^sub>A = (stack_to_mem (i1 # i2 # \<sigma>) \<mu>, Some 0, d, 
+      [CAssm {A} (Reg M), CAssm {D} (Reg M), AAssm 0, 
+       CAssm {A, M} (Decr M), CAssm {M} DAndM, AAssm 0] @ ?\<pi>')" by fastforce
+    from 7 have S: "\<Sigma>\<^sub>S' = (unboolify (boolify i1 \<and> boolify i2) # \<sigma>, \<pi>)" by simp
+    let ?\<mu> = "stack_to_mem (i1 # i2 # \<sigma>) \<mu>"
+    let ?\<mu>' = "stack_to_mem (unboolify (boolify i1 \<and> boolify i2) # \<sigma>) ?\<mu>"
+    let ?\<Sigma>\<^sub>A\<^sub>1 = "(?\<mu>, Some (?\<mu> 0), d, 
+      [CAssm {D} (Reg M), AAssm 0, CAssm {A, M} (Decr M), CAssm {M} DAndM, AAssm 0] @ ?\<pi>')"
+    let ?\<Sigma>\<^sub>A\<^sub>2 = "(?\<mu>, Some (?\<mu> 0), ?\<mu> (?\<mu> 0), 
+      [AAssm 0, CAssm {A, M} (Decr M), CAssm {M} DAndM, AAssm 0] @ ?\<pi>')"
+    let ?\<Sigma>\<^sub>A\<^sub>3 = "(?\<mu>, Some 0, ?\<mu> (?\<mu> 0), [CAssm {A, M} (Decr M), CAssm {M} DAndM, AAssm 0] @ ?\<pi>')"
+    let ?\<Sigma>\<^sub>A\<^sub>4 = "(?\<mu>(0 := ?\<mu> 0 - 1), Some (?\<mu> 0 - 1), ?\<mu> (?\<mu> 0), [CAssm {M} DAndM, AAssm 0] @ ?\<pi>')"
+    let ?\<Sigma>\<^sub>A\<^sub>5 = "(?\<mu>', Some (?\<mu> 0 - 1), ?\<mu> (?\<mu> 0), [AAssm 0] @ ?\<pi>')"
+    let ?\<Sigma>\<^sub>A\<^sub>6 = "(?\<mu>', Some 0, ?\<mu> (?\<mu> 0), ?\<pi>')"
+    from M have step1: "eval_assembly (program_convert \<Pi>) \<Sigma>\<^sub>A = Some ?\<Sigma>\<^sub>A\<^sub>1" by simp
+    have step2: "eval_assembly (program_convert \<Pi>) ?\<Sigma>\<^sub>A\<^sub>1 = Some ?\<Sigma>\<^sub>A\<^sub>2" by simp
+    have step3: "eval_assembly (program_convert \<Pi>) ?\<Sigma>\<^sub>A\<^sub>2 = Some ?\<Sigma>\<^sub>A\<^sub>3" by simp
+    have step4: "eval_assembly (program_convert \<Pi>) ?\<Sigma>\<^sub>A\<^sub>3 = Some ?\<Sigma>\<^sub>A\<^sub>4" by (simp add: Let_def)
+    have step5: "eval_assembly (program_convert \<Pi>) ?\<Sigma>\<^sub>A\<^sub>4 = Some ?\<Sigma>\<^sub>A\<^sub>5" by simp
+    have step6: "eval_assembly (program_convert \<Pi>) ?\<Sigma>\<^sub>A\<^sub>5 = Some ?\<Sigma>\<^sub>A\<^sub>6" by simp
+    from iter_two iter_prestep step1 step2 step3 have
+      "iterate (eval_assembly (program_convert \<Pi>)) \<Sigma>\<^sub>A ?\<Sigma>\<^sub>A\<^sub>3" by fast
+    moreover from iter_two iter_prestep step4 step5 step6 have
+      "iterate (eval_assembly (program_convert \<Pi>)) ?\<Sigma>\<^sub>A\<^sub>3 ?\<Sigma>\<^sub>A\<^sub>6" by fast
+    ultimately have X: "iterate (eval_assembly (program_convert \<Pi>)) \<Sigma>\<^sub>A ?\<Sigma>\<^sub>A\<^sub>6" by fast
+    have "?\<Sigma>\<^sub>A\<^sub>6 \<in> state_convert (unboolify (boolify i1 \<and> boolify i2) # \<sigma>, \<pi>)" by auto
+    with X S M show ?case by metis
+  next case (8 \<Pi> i1 i2 \<sigma> \<pi>)
+    let ?\<pi>' = "concat (map instruction_conv \<pi>)"
+    from 8 obtain d \<mu> where M: "\<Sigma>\<^sub>A = (stack_to_mem (i1 # i2 # \<sigma>) \<mu>, Some 0, d, 
+      [CAssm {A} (Reg M), CAssm {D} (Reg M), AAssm 0, 
+       CAssm {A, M} (Decr M), CAssm {M} DOrM, AAssm 0] @ ?\<pi>')" by fastforce
+    from 8 have S: "\<Sigma>\<^sub>S' = (unboolify (boolify i1 \<or> boolify i2) # \<sigma>, \<pi>)" by simp
+    let ?\<mu> = "stack_to_mem (i1 # i2 # \<sigma>) \<mu>"
+    let ?\<mu>' = "stack_to_mem (unboolify (boolify i1 \<or> boolify i2) # \<sigma>) ?\<mu>"
+    let ?\<Sigma>\<^sub>A\<^sub>1 = "(?\<mu>, Some (?\<mu> 0), d, 
+      [CAssm {D} (Reg M), AAssm 0, CAssm {A, M} (Decr M), CAssm {M} DOrM, AAssm 0] @ ?\<pi>')"
+    let ?\<Sigma>\<^sub>A\<^sub>2 = "(?\<mu>, Some (?\<mu> 0), ?\<mu> (?\<mu> 0), 
+      [AAssm 0, CAssm {A, M} (Decr M), CAssm {M} DOrM, AAssm 0] @ ?\<pi>')"
+    let ?\<Sigma>\<^sub>A\<^sub>3 = "(?\<mu>, Some 0, ?\<mu> (?\<mu> 0), [CAssm {A, M} (Decr M), CAssm {M} DOrM, AAssm 0] @ ?\<pi>')"
+    let ?\<Sigma>\<^sub>A\<^sub>4 = "(?\<mu>(0 := ?\<mu> 0 - 1), Some (?\<mu> 0 - 1), ?\<mu> (?\<mu> 0), [CAssm {M} DOrM, AAssm 0] @ ?\<pi>')"
+    let ?\<Sigma>\<^sub>A\<^sub>5 = "(?\<mu>', Some (?\<mu> 0 - 1), ?\<mu> (?\<mu> 0), [AAssm 0] @ ?\<pi>')"
+    let ?\<Sigma>\<^sub>A\<^sub>6 = "(?\<mu>', Some 0, ?\<mu> (?\<mu> 0), ?\<pi>')"
+    from M have step1: "eval_assembly (program_convert \<Pi>) \<Sigma>\<^sub>A = Some ?\<Sigma>\<^sub>A\<^sub>1" by simp
+    have step2: "eval_assembly (program_convert \<Pi>) ?\<Sigma>\<^sub>A\<^sub>1 = Some ?\<Sigma>\<^sub>A\<^sub>2" by simp
+    have step3: "eval_assembly (program_convert \<Pi>) ?\<Sigma>\<^sub>A\<^sub>2 = Some ?\<Sigma>\<^sub>A\<^sub>3" by simp
+    have step4: "eval_assembly (program_convert \<Pi>) ?\<Sigma>\<^sub>A\<^sub>3 = Some ?\<Sigma>\<^sub>A\<^sub>4" by (simp add: Let_def)
+    have step5: "eval_assembly (program_convert \<Pi>) ?\<Sigma>\<^sub>A\<^sub>4 = Some ?\<Sigma>\<^sub>A\<^sub>5" by simp
+    have step6: "eval_assembly (program_convert \<Pi>) ?\<Sigma>\<^sub>A\<^sub>5 = Some ?\<Sigma>\<^sub>A\<^sub>6" by simp
+    from iter_two iter_prestep step1 step2 step3 have
+      "iterate (eval_assembly (program_convert \<Pi>)) \<Sigma>\<^sub>A ?\<Sigma>\<^sub>A\<^sub>3" by fast
+    moreover from iter_two iter_prestep step4 step5 step6 have
+      "iterate (eval_assembly (program_convert \<Pi>)) ?\<Sigma>\<^sub>A\<^sub>3 ?\<Sigma>\<^sub>A\<^sub>6" by fast
+    ultimately have X: "iterate (eval_assembly (program_convert \<Pi>)) \<Sigma>\<^sub>A ?\<Sigma>\<^sub>A\<^sub>6" by fast
+    have "?\<Sigma>\<^sub>A\<^sub>6 \<in> state_convert (unboolify (boolify i1 \<or> boolify i2) # \<sigma>, \<pi>)" by auto
+    with X S M show ?case by metis
+  next case (9 \<Pi> i1 \<sigma> \<pi>)
+    let ?\<pi>' = "concat (map instruction_conv \<pi>)"
+    from 9 obtain d \<mu> where M: "\<Sigma>\<^sub>A = (stack_to_mem (i1 # \<sigma>) \<mu>, Some 0, d, 
+      [CAssm {A} (Reg M), CAssm {M} (NotR M), AAssm 0] @ ?\<pi>')" by fastforce
+    from 9 have S: "\<Sigma>\<^sub>S' = (unboolify (\<not> boolify i1) # \<sigma>, \<pi>)" by simp
+    let ?\<mu> = "stack_to_mem (i1 # \<sigma>) \<mu>"
+    let ?\<Sigma>\<^sub>A\<^sub>1 = "(?\<mu>, Some (?\<mu> 0), d, [CAssm {M} (NotR M), AAssm 0] @ ?\<pi>')"
+    let ?\<Sigma>\<^sub>A\<^sub>2 = "(?\<mu>(?\<mu> 0 := unboolify (\<not> boolify (?\<mu> (?\<mu> 0)))), Some (?\<mu> 0), d, [AAssm 0] @ ?\<pi>')"
+    let ?\<Sigma>\<^sub>A\<^sub>3 = "(?\<mu>(?\<mu> 0 := unboolify (\<not> boolify (?\<mu> (?\<mu> 0)))), Some 0, d, ?\<pi>')"
+    from M have step1: "eval_assembly (program_convert \<Pi>) \<Sigma>\<^sub>A = Some ?\<Sigma>\<^sub>A\<^sub>1" by simp
+    have step2: "eval_assembly (program_convert \<Pi>) ?\<Sigma>\<^sub>A\<^sub>1 = Some ?\<Sigma>\<^sub>A\<^sub>2" by simp
+    have "eval_assembly (program_convert \<Pi>) ?\<Sigma>\<^sub>A\<^sub>2 = Some ?\<Sigma>\<^sub>A\<^sub>3" by simp
+    with iter_two iter_prestep step1 step2 have X:
+      "iterate (eval_assembly (program_convert \<Pi>)) \<Sigma>\<^sub>A ?\<Sigma>\<^sub>A\<^sub>3" by fast
+    have "(stack_to_mem (i1 # \<sigma>) \<mu>)(1 + int (length \<sigma>) := unboolify (\<not> boolify i1)) = 
+      stack_to_mem (unboolify (\<not> boolify i1) # \<sigma>) \<mu>" by auto
+    hence "?\<Sigma>\<^sub>A\<^sub>3 \<in> state_convert (unboolify (\<not> boolify i1) # \<sigma>, \<pi>)" by auto
+    with X S M show ?case by metis
+  next 
 
   (* autogenerated cases where "eval_stack \<Pi> \<Sigma>\<^sub>S = None" *)
-  next case "10_1" thus ?case by simp
+  case "10_1" thus ?case by simp
   next case "10_2" thus ?case by simp
   next case "10_3" thus ?case by simp
   next case "10_4" thus ?case by simp
